NonEmpty/CorrectByConstruction/Array/MapIdx.lean
@@ -78,12 +78,14 @@ theorem mapFinIdx_spec {xs : NonEmptyArray α} {f : (i : Nat) → α → (h : i 
   (mapFinIdx_induction (motive := fun _ => True) (h0 := trivial) (hs := fun i h _ => ⟨hs i h, trivial⟩)).2
 
 @[simp, grind =] theorem size_zipIdx {xs : NonEmptyArray α} {k : Nat} : (xs.zipIdx k).size = xs.size := by
-  simp [zipIdx, size]
+  simp only [size, zipIdx, _root_.Array.size_zipIdx]
 
 @[simp, grind =] theorem getElem_mapFinIdx {xs : NonEmptyArray α} {f : (i : Nat) → α → (h : i < xs.size) → β} {i : Nat}
     (h : i < (xs.mapFinIdx f).size) :
-    (xs.mapFinIdx f)[i] = f i (xs[i]'(by simp_all [size_mapFinIdx])) (by simp_all [size_mapFinIdx]) :=
-  (mapFinIdx_spec (p := fun i b h => b = f i xs[i] h) fun _ _ => rfl).2 i (by simp_all [size_mapFinIdx])
+    (xs.mapFinIdx f)[i] = f i (xs[i]'(by simp_all only [size, size_mapFinIdx])) (by simp_all only [size,
+      size_mapFinIdx]) :=
+  (mapFinIdx_spec (p := fun i b h => b = f i xs[i] h) fun _ _ => rfl).2 i (by simp_all only [size,
+    size_mapFinIdx])
 
 @[simp, grind =] theorem getElem?_mapFinIdx {xs : NonEmptyArray α} {f : (i : Nat) → α → (h : i < xs.size) → β} {i : Nat} :
     (xs.mapFinIdx f)[i]? =
@@ -99,7 +101,7 @@ theorem mapFinIdx_spec {xs : NonEmptyArray α} {f : (i : Nat) → α → (h : i 
   · unfold size toList mapFinIdx; simp only [_root_.Array.toList_mapFinIdx, Array.length_toList,
     List.length_cons, List.length_mapFinIdx, List.mapFinIdx_cons]
   · intro i h1 h2
-    simp [toList, mapFinIdx]
+    simp only [toList, mapFinIdx, _root_.Array.toList_mapFinIdx, Array.length_toList, List.length_cons, List.mapFinIdx_cons]
 
 /-! ### mapIdx -/
 
@@ -122,22 +124,26 @@ theorem mapIdx_spec {f : Nat → α → β} {xs : NonEmptyArray α}
 
 @[simp, grind =] theorem getElem_mapIdx {f : Nat → α → β} {xs : NonEmptyArray α} {i : Nat}
     (h : i < (xs.mapIdx f).size) :
-    (xs.mapIdx f)[i] = f i (xs[i]'(by simp_all [size_mapIdx])) :=
-  (mapIdx_spec (p := fun i b h => b = f i xs[i]) fun _ _ => rfl).2 i (by simp_all [size_mapIdx])
+    (xs.mapIdx f)[i] = f i (xs[i]'(by simp_all only [size, size_mapIdx])) :=
+  (mapIdx_spec (p := fun i b h => b = f i xs[i]) fun _ _ => rfl).2 i (by simp_all only [size,
+    size_mapIdx])
 
 @[simp, grind =] theorem getElem?_mapIdx {f : Nat → α → β} {xs : NonEmptyArray α} {i : Nat} :
     (xs.mapIdx f)[i]? =
       xs[i]?.map (f i) := by
-  simp [getElem?_def, size_mapIdx, getElem_mapIdx]
+  simp only [size, getElem?_def, size_mapIdx, getElem_mapIdx, Option.map_dif]
 
 @[simp, grind =] theorem toList_mapIdx {f : Nat → α → β} {xs : NonEmptyArray α} :
     (xs.mapIdx f).toList = xs.toList.mapIdx (fun i a => f i a) := by
   apply List.ext_getElem
-  · simp [mapIdx]
+  · simp only [toList, mapIdx, _root_.Array.toList_mapIdx, List.length_cons, List.length_mapIdx,
+    Array.length_toList, List.mapIdx_cons]
   · intro i h1 h2
     cases i with
-    | zero => simp [mapIdx]
-    | succ i => simp [mapIdx]
+    | zero => simp only [toList, mapIdx, _root_.Array.toList_mapIdx, List.getElem_cons_zero,
+      List.mapIdx_cons]
+    | succ i => simp only [toList, mapIdx, _root_.Array.toList_mapIdx, List.getElem_cons_succ,
+      List.getElem_mapIdx, Array.getElem_toList, List.mapIdx_cons]
 
 /-! ### zipIdx -/
 
@@ -153,15 +159,18 @@ theorem mapIdx_spec {f : Nat → α → β} {xs : NonEmptyArray α}
 
 @[simp, grind =] theorem zipIdx_toArr {xs : NonEmptyArray α} {k : Nat} :
     (xs.zipIdx k).toArr = xs.toArr.zipIdx k := by
-  simp [zipIdx, toArr, Array.zipIdx_append]
+  simp only [toArr, zipIdx, Array.zipIdx_append, Array.zipIdx_toArray, List.zipIdx_cons,
+    List.zipIdx_nil, List.size_toArray, List.length_cons, List.length_nil, Nat.zero_add]
 
 @[simp, grind =] theorem toList_zipIdx {xs : NonEmptyArray α} {k : Nat} :
     (xs.zipIdx k).toList = xs.toList.zipIdx k := by
-  simp [zipIdx]
+  simp only [toList, zipIdx, _root_.Array.toList_zipIdx, List.zipIdx_cons]
 
 theorem mk_mem_zipIdx_iff_le_and_getElem?_sub {k i : Nat} {x : α} {xs : NonEmptyArray α} :
     (x, i) ∈ xs.zipIdx k ↔ k ≤ i ∧ xs[i - k]? = some x := by
-  simp [mem_def, zipIdx_toArr, _root_.Array.mk_mem_zipIdx_iff_le_and_getElem?_sub, GetElem?.getElem?]
+  simp only [mem_def, toArr, zipIdx_toArr, _root_.Array.mk_mem_zipIdx_iff_le_and_getElem?_sub,
+    getElem?, Option.dite_none_right_eq_some, Option.some.injEq, Array.size_append,
+    List.size_toArray, List.length_cons, List.length_nil, Nat.zero_add, size, and_congr_right_iff]
   intro a
   simp_all only [size, toArr_getElem]
   rfl
@@ -174,7 +183,7 @@ theorem mk_mem_zipIdx_iff_getElem? {x : α} {i : Nat} {xs : NonEmptyArray α} :
 theorem mem_zipIdx_iff_le_and_getElem?_sub {x : α × Nat} {xs : NonEmptyArray α} {k : Nat} :
     x ∈ xs.zipIdx k ↔ k ≤ x.2 ∧ xs[x.2 - k]? = some x.1 := by
   cases x
-  simp [mk_mem_zipIdx_iff_le_and_getElem?_sub]
+  simp only [mk_mem_zipIdx_iff_le_and_getElem?_sub, size]
 
 theorem mem_zipIdx_iff_getElem? {x : α × Nat} {xs : NonEmptyArray α} :
     x ∈ xs.zipIdx ↔ xs[x.2]? = some x.1 := by
@@ -184,83 +193,207 @@ theorem mem_zipIdx_iff_getElem? {x : α × Nat} {xs : NonEmptyArray α} :
 
 @[congr] theorem mapFinIdx_congr {xs ys : NonEmptyArray α} (w : xs = ys)
     (f : (i : Nat) → α → (h : i < xs.size) → β) :
-    xs.mapFinIdx f = ys.mapFinIdx (fun i a h => f i a (by simp [w]; omega)) := by
+    xs.mapFinIdx f = ys.mapFinIdx (fun i a h => f i a (by simp only [size, w]; omega)) := by
   subst w
   rfl
 
 theorem mapFinIdx_eq_ofFn {xs : NonEmptyArray α} {f : (i : Nat) → α → (h : i < xs.size) → β} :
     xs.mapFinIdx f = NonEmptyArray.ofFn (n := xs.tail.size) fun i =>
-      f i.val (xs[i.val]'(by simp [size]; omega)) (by simp [size]; omega) := by
+      f i.val (xs[i.val]'(by simp only [size]; omega)) (by simp only [size]; omega) := by
   apply toArr_inj.1
-  simp [toArr_mapFinIdx, toArr_ofFn, _root_.Array.mapFinIdx_eq_ofFn]
+  simp only [toArr, toArr_mapFinIdx, _root_.Array.mapFinIdx_eq_ofFn, Fin.getElem_fin, size,
+    toArr_ofFn]
   apply Array.ext
   · simp at *; omega
   · intro i h1 h2
-    simp [_root_.Array.getElem_ofFn]
-    rw [toArr_getElem xs i (by simp [size] at *; omega)]
+    simp only [Array.getElem_ofFn]
+    rw [toArr_getElem xs i (by simp only [Array.size_ofFn, Array.size_append, List.size_toArray,
+      List.length_cons, List.length_nil, Nat.zero_add, size] at *; omega)]
 
--- @[grind =]
--- theorem mapFinIdx_append {xs ys : NonEmptyArray α} {f : (i : Nat) → α → (h : i < (xs ++ ys).size) → β} :
---     (xs ++ ys).mapFinIdx f =
---       xs.mapFinIdx (fun i a h => f i a (by simp; grind only)) ++
---         ys.mapFinIdx (fun i a h => f (i + xs.size) a (by simp; grind only)) := by
---   apply toArr_inj.1
---   simp [toArr_mapFinIdx, toArr_append, Array.mapFinIdx_append]
+@[grind =]
+theorem mapFinIdx_append {xs ys : NonEmptyArray α} {f : (i : Nat) → α → (h : i < (xs ++ ys).size) → β} :
+    (xs ++ ys).mapFinIdx f =
+      xs.mapFinIdx (fun i a h => f i a (by simp; grind only)) ++
+        ys.mapFinIdx (fun i a h => f (i + xs.size) a (by simp; grind only)) := by
+  apply toArr_inj.1
+  simp only [toArr, toArr_mapFinIdx, toArr_append, Array.append_singleton_assoc, Array.push_append,
+    Array.append_assoc, _root_.Array.mapFinIdx_append, List.mapFinIdx_toArray, List.mapFinIdx_cons,
+    List.length_nil, List.mapFinIdx_nil,
+    List.size_toArray, List.length_cons, Nat.zero_add, Array.mapFinIdx_push, Array.size_push, size]
+  simp_all only [Nat.add_comm, Nat.add_left_comm, Nat.reduceAdd]
 
--- @[simp, grind =]
--- theorem mapFinIdx_push {xs : NonEmptyArray α} {a : α} {f : (i : Nat) → α → (h : i < (xs.push a).size) → β} :
---     mapFinIdx (xs.push a) f =
---       (mapFinIdx xs (fun i a h => f i a (by
---         simp;
---         simp_all only [size]
---         aesop?)
---       )).push (f xs.size a (by
---         simp_all only [size, Nat.add_lt_add_iff_left]
---         aesop?)
---       ) := by
---   ext <;> simp [mapFinIdx, toArr, Array.mapFinIdx_push]
+@[simp, grind =]
+theorem mapFinIdx_push {xs : NonEmptyArray α} {a : α} {f : (i : Nat) → α → (h : i < (xs.push a).size) → β} :
+    mapFinIdx (xs.push a) f =
+      (mapFinIdx xs (fun i a h => f i a (by simp only [size, push, Array.size_push] at *; omega))).push (f xs.size a (by simp only [size,
+        push, Array.size_push, Nat.add_lt_add_iff_left, Nat.lt_add_one] at *)) := by
+  apply toArr_inj.1
+  apply Array.ext
+  · simp only [toArr, push, _root_.Array.size_mapFinIdx, Array.size_append,
+    List.size_toArray, List.length_cons, List.length_nil, Nat.zero_add, Array.size_push, size,
+    mapFinIdx_tail] at *
+  · intro i h1 h2
+    simp only [toArr, mapFinIdx, push, _root_.Array.mapFinIdx_push, Array.getElem_append,
+      List.size_toArray, List.length_cons, List.length_nil, Nat.zero_add, Nat.lt_one_iff,
+      List.getElem_toArray, List.getElem_singleton, Array.getElem_push, _root_.Array.size_mapFinIdx,
+      _root_.Array.getElem_mapFinIdx, dite_eq_ite, size] at *
+    repeat split
+    all_goals (congr <;> (simp only [toArr, push, toArr_mapFinIdx, _root_.Array.size_mapFinIdx,
+      Array.size_append, List.size_toArray, List.length_cons, List.length_nil, Nat.zero_add,
+      Array.size_push, size] at *; grind only))
 
 theorem mapFinIdx_singleton {a : α} {f : (i : Nat) → α → (h : i < 1) → β} :
     (NonEmptyArray.singleton a).mapFinIdx f = NonEmptyArray.singleton (f 0 a (by simp)) := by
-  simp [NonEmptyArray.singleton, mapFinIdx]
+  simp only [mapFinIdx, NonEmptyArray.singleton, List.mapFinIdx_toArray,
+    List.mapFinIdx_nil]
 
--- theorem mapFinIdx_eq_zipIdx_map {xs : NonEmptyArray α} {f : (i : Nat) → α → (h : i < xs.size) → β} :
---     xs.mapFinIdx f = xs.zipIdx.attach.map
---       fun ⟨⟨x, i⟩, m⟩ =>
---         f i x (by simp [mk_mem_zipIdx_iff_getElem?, getElem?_eq_some_iff] at m; exact m.1) := by
---   ext <;> simp
+theorem mapFinIdx_eq_zipIdx_map {xs : NonEmptyArray α} {f : (i : Nat) → α → (h : i < xs.size) → β} :
+    xs.mapFinIdx f = xs.zipIdx.attach.map
+      fun ⟨⟨x, i⟩, m⟩ =>
+        f i x (by simp only [mk_mem_zipIdx_iff_getElem?, size, getElem?_eq_some_iff] at m; exact m.1) := by
+  ext
+  · simp_all only [attach]
+    rfl
+  · simp only [mapFinIdx, _root_.Array.size_mapFinIdx, zipIdx, Nat.reduceAdd, attach, Nat.zero_add,
+    Array.map_map, Array.size_map, Array.size_attach, _root_.Array.size_zipIdx]
+  · simp only [mapFinIdx, _root_.Array.getElem_mapFinIdx, zipIdx, Nat.reduceAdd, attach,
+    Nat.zero_add, Array.map_map, Array.getElem_map, Array.getElem_attach,
+    _root_.Array.getElem_zipIdx, Nat.add_comm, Function.comp_apply]
 
+theorem exists_of_mem_mapFinIdx {b : β} {xs : NonEmptyArray α} {f : (i : Nat) → α → (h : i < xs.size) → β}
+    (h : b ∈ xs.mapFinIdx f) : ∃ (i : Nat) (h : i < xs.size), f i xs[i] h = b := by
+  have h' := h
+  rw [mem_def, toArr_mapFinIdx] at h'
+  obtain ⟨i, hi, h_eq⟩ := _root_.Array.exists_of_mem_mapFinIdx h'
+  refine ⟨i, by simpa using hi, ?_⟩
+  rw [← h_eq]
+  congr 1
+  · subst h_eq
+    simp_all only [toArr, Array.mem_mapFinIdx, Array.size_append, List.size_toArray, List.length_cons, List.length_nil,
+      Nat.zero_add, size, toArr_getElem]
+    obtain ⟨w, h_1⟩ := h'
+    obtain ⟨w_1, h_1⟩ := h_1
+    aesop?
 
+@[simp, grind =] theorem mem_mapFinIdx {b : β} {xs : NonEmptyArray α} {f : (i : Nat) → α → (h : i < xs.size) → β} :
+    b ∈ xs.mapFinIdx f ↔ ∃ (i : Nat) (h : i < xs.size), f i xs[i] h = b := by
+  constructor
+  · intro h; exact exists_of_mem_mapFinIdx h
+  · intro a
+    simp_all only [size]
+    obtain ⟨w, h⟩ := a
+    obtain ⟨w_1, h⟩ := h
+    subst h
+    aesop?
 
--- theorem exists_of_mem_mapFinIdx {b : β} {xs : NonEmptyArray α} {f : (i : Nat) → α → (h : i < xs.size) → β}
---     (h : b ∈ xs.mapFinIdx f) : ∃ (i : Nat) (h : i < xs.size), f i xs[i] h = b := by
---   simp [mem_def, toArr_mapFinIdx] at h
---   exact Array.exists_of_mem_mapFinIdx h
+theorem mapFinIdx_eq_iff {xs : NonEmptyArray α} {f : (i : Nat) → α → (h : i < xs.size) → β} {ys : NonEmptyArray β} :
+    xs.mapFinIdx f = ys ↔ ys.size = xs.size ∧ ∀ (i : Nat) (hi : i < xs.size), ys[i]'(by
+    simp_all only [size]
+    aesop?) = f i xs[i] hi := by
+  rw [← toArr_inj, toArr_mapFinIdx, _root_.Array.mapFinIdx_eq_iff]
+  simp only [toArr, Array.size_append, List.size_toArray, List.length_cons, List.length_nil,
+    Nat.zero_add, Nat.add_left_cancel_iff, size]
+  constructor
+  · rintro ⟨hsz, h⟩
+    refine ⟨hsz, ?_⟩
+    intro i hi
+    specialize h i hi
+    simp_all only [size, toArr_getElem]
+  · rintro ⟨hsz, h⟩
+    refine ⟨hsz, ?_⟩
+    intro i hi
+    specialize h i hi
+    simp_all only [size, toArr_getElem]
 
--- @[simp, grind =] theorem mem_mapFinIdx {b : β} {xs : NonEmptyArray α} {f : (i : Nat) → α → (h : i < xs.size) → β} :
---     b ∈ xs.mapFinIdx f ↔ ∃ (i : Nat) (h : i < xs.size), f i xs[i] h = b := by
---   simp [mem_def, toArr_mapFinIdx, Array.mem_mapFinIdx]
+@[simp] theorem mapFinIdx_eq_singleton_iff {xs : NonEmptyArray α} {f : (i : Nat) → α → (h : i < xs.size) → β} {b : β} :
+    xs.mapFinIdx f = NonEmptyArray.singleton b ↔ ∃ (a : α) (w : xs = NonEmptyArray.singleton a), f 0 a (by aesop) = b := by
+  rw [← toArr_inj, toArr_mapFinIdx, NonEmptyArray.toArr_singleton, _root_.Array.mapFinIdx_eq_singleton_iff]
+  simp only [toArr, Array.append_eq_toArray_iff, List.cons_append, List.nil_append, List.cons.injEq,
+    Array.toList_eq_nil_iff]
+  aesop
 
--- theorem mapFinIdx_eq_iff {xs : NonEmptyArray α} {f : (i : Nat) → α → (h : i < xs.size) → β} {ys : NonEmptyArray β} :
---     xs.mapFinIdx f = ys ↔ ∀ (i : Nat) (h : i < xs.size), ys[i] = f i xs[i] h := by
---   ext <;> simp
+theorem mapFinIdx_eq_append_iff {xs : NonEmptyArray α} {f : (i : Nat) → α → (h : i < xs.size) → β} {ys zs : NonEmptyArray β} :
+    xs.mapFinIdx f = ys ++ zs ↔
+      ∃ (ys' : NonEmptyArray α) (zs' : NonEmptyArray α) (w : xs = ys' ++ zs'),
+        ys'.mapFinIdx (fun i a h => f i a (by
+          simp only [size, w, size_append]
+          subst w
+          simp_all only [size]
+          aesop?)) = ys ∧
+        zs'.mapFinIdx (fun i a h => f (i + ys'.size) a (by
+          simp only [size, w, size_append]
+          subst w
+          simp_all only [size]
+          aesop?)) = zs := by
+  rw [← toArr_inj, toArr_mapFinIdx, toArr_append, _root_.Array.mapFinIdx_eq_append_iff]
+  constructor
+  · rintro ⟨ys', zs', w, h1, h2⟩
+    have hys : ys'.size > 0 := by
+      have := congrArg Array.size w;
+      simp at this;
+      simp_all only [toArr, gt_iff_lt]
+      aesop?
+    have hzs : zs'.size > 0 := by
+      have := congrArg Array.size w;
+      simp at this;
+      simp_all only [toArr, gt_iff_lt]
+      aesop?
+    refine ⟨⟨ys'[0], ys'[1:]⟩, ⟨zs'[0], zs'[1:]⟩, ?_, ?_, ?_⟩
+    · simp_all only [toArr, Subarray.copy_eq_toArray]
+      aesop?
+    · simp_all only [toArr, Subarray.copy_eq_toArray, size]
+      aesop?
+    · simp_all only [toArr, Subarray.copy_eq_toArray, size, Std.Slice.size_toArray_eq_size]
+      aesop?
+  · intro a
+    simp_all only [size, toArr]
+    obtain ⟨w, h⟩ := a
+    obtain ⟨w_1, h⟩ := h
+    obtain ⟨w_2, h⟩ := h
+    obtain ⟨left, right⟩ := h
+    subst w_2 left right
+    simp_all only [toArr_mapFinIdx, toArr, toArr_append, Array.append_singleton_assoc, Array.push_append,
+      Array.append_assoc]
+    apply Exists.intro
+    · apply Exists.intro
+      · apply Exists.intro
+        · apply And.intro
+          · rfl
+          · simp_all only [Array.size_append, List.size_toArray, List.length_cons, List.length_nil, Nat.zero_add]
+            rfl
+        · simp_all only [Array.append_singleton_assoc, Array.push_append, Array.append_assoc]
 
--- @[simp] theorem mapFinIdx_eq_singleton_iff {xs : NonEmptyArray α} {f : (i : Nat) → α → (h : i < xs.size) → β} {b : β} :
---     xs.mapFinIdx f = NonEmptyArray.singleton b ↔ ∃ (a : α) (w : xs = NonEmptyArray.singleton a), f 0 a (by aesop?) = b := by
---   ext <;> simp [mapFinIdx, toArr, Array.mapFinIdx_eq_singleton_iff]
-
--- theorem mapFinIdx_eq_append_iff {xs : NonEmptyArray α} {f : (i : Nat) → α → (h : i < xs.size) → β} {ys zs : NonEmptyArray β} :
---     xs.mapFinIdx f = ys ++ zs ↔
---       ∃ (ys' : NonEmptyArray α) (zs' : NonEmptyArray α) (w : xs = ys' ++ zs'),
---         ys'.mapFinIdx (fun i a h => f i a (by simp [w]; grind only)) = ys ∧
---         zs'.mapFinIdx (fun i a h => f (i + ys'.size) a (by simp [w]; grind only)) = zs := by
---   ext <;> simp [mapFinIdx, toArr, Array.mapFinIdx_eq_append_iff]
-
--- theorem mapFinIdx_eq_push_iff {xs : NonEmptyArray α} {b : β} {f : (i : Nat) → α → (h : i < xs.size) → β} :
---     xs.mapFinIdx f = ys.push b ↔
---       ∃ (zs : NonEmptyArray α) (a : α) (w : xs = zs.push a),
---         zs.mapFinIdx (fun i a h => f i a (by simp [w]; aesop?)) = ys ∧ b = f (xs.size - 1) a (by simp [w]) := by
---   ext <;> simp [mapFinIdx, toArr, Array.mapFinIdx_eq_push_iff]
+theorem mapFinIdx_eq_push_iff {xs : NonEmptyArray α} {b : β} {f : (i : Nat) → α → (h : i < xs.size) → β} :
+    xs.mapFinIdx f = ys.push b ↔
+      ∃ (zs : NonEmptyArray α) (a : α) (w : xs = zs.push a),
+        zs.mapFinIdx (fun i a h => f i a (by
+          simp only [size, w];
+          subst w
+          simp_all only [size]
+          aesop?)
+          ) = ys ∧ b = f (xs.size - 1) a (by simp only [size, w, Nat.add_sub_cancel_left,
+            Nat.lt_add_left_iff_pos, Nat.lt_add_one]) := by
+  rw [← toArr_inj, toArr_mapFinIdx, toArr_push, _root_.Array.mapFinIdx_eq_push_iff]
+  constructor
+  · rintro ⟨zs, a, w, h1, h2⟩
+    have hzs : zs.size > 0 := by
+      have := congrArg Array.size w; simp at this;
+      subst h2
+      simp_all only [toArr, gt_iff_lt]
+      aesop?
+    refine ⟨⟨zs[0], zs[1:]⟩, a, ?_, ?_, ?_⟩
+    · subst h2
+      simp_all only [toArr, Subarray.copy_eq_toArray]
+      aesop?
+    · subst h2
+      simp_all only [toArr, Subarray.copy_eq_toArray, size]
+      aesop?
+    · simp only [h2, toArr, Array.size_append, List.size_toArray, List.length_cons,
+      List.length_nil, Nat.zero_add, Nat.add_sub_cancel_left, size]
+  · rintro ⟨zs, a, rfl, rfl, rfl⟩
+    simp_all only [toArr, size, toArr_mapFinIdx, Nat.add_sub_cancel_left, Array.size_push, Nat.add_one_sub_one,
+      toArr_push, Array.push_append]
+    aesop?
 
 -- theorem mapFinIdx_eq_mapFinIdx_iff {xs : NonEmptyArray α} {f g : (i : Nat) → α → (h : i < xs.size) → β} :
 --     xs.mapFinIdx f = xs.mapFinIdx g ↔ ∀ (i : Nat) (h : i < xs.size), f i xs[i] h = g i xs[i] h := by
@@ -300,7 +433,7 @@ theorem mapFinIdx_singleton {a : α} {f : (i : Nat) → α → (h : i < 1) → �
 
 -- theorem mapIdx_eq_mapFinIdx {xs : NonEmptyArray α} {f : Nat → α → β} :
 --     xs.mapIdx f = xs.mapFinIdx (fun i a _ => f i a) := by
---   simp [mapFinIdx_eq_mapIdx]
+--   simp? [mapFinIdx_eq_mapIdx]
 
 -- theorem mapIdx_eq_zipIdx_map {xs : NonEmptyArray α} {f : Nat → α → β} :
 --     xs.mapIdx f = xs.zipIdx.map fun ⟨a, i⟩ => f i a := by
@@ -319,39 +452,39 @@ theorem mapFinIdx_singleton {a : α} {f : (i : Nat) → α → (h : i < 1) → �
 -- @[simp, grind =]
 -- theorem mapIdx_push {xs : NonEmptyArray α} {a : α} :
 --     mapIdx f (xs.push a) = (mapIdx f xs).push (f xs.size a) := by
---   ext <;> simp [mapIdx, toArr, Array.mapIdx_push]
+--   ext <;> simp? [mapIdx, toArr, Array.mapIdx_push]
 
 -- theorem mapIdx_singleton {a : α} : mapIdx f (NonEmptyArray.singleton a) = NonEmptyArray.singleton (f 0 a) := by
---   simp [NonEmptyArray.singleton, mapIdx, mapIdxM, mapFinIdxM]
+--   simp? [NonEmptyArray.singleton, mapIdx, mapIdxM, mapFinIdxM]
 
 -- @[simp]
 -- theorem mapIdx_eq_singleton_iff {xs : NonEmptyArray α} {f : Nat → α → β} {b : β} :
 --     mapIdx f xs = NonEmptyArray.singleton b ↔ ∃ (a : α), xs = NonEmptyArray.singleton a ∧ f 0 a = b := by
---   ext <;> simp [mapIdx, toArr, Array.mapIdx_eq_singleton_iff]
+--   ext <;> simp? [mapIdx, toArr, Array.mapIdx_eq_singleton_iff]
 
 -- theorem exists_of_mem_mapIdx {b : β} {xs : NonEmptyArray α}
 --     (h : b ∈ mapIdx f xs) : ∃ (i : Nat) (h : i < xs.size), f i xs[i] = b := by
---   simp [mem_def, toArr, mapIdx] at h
+--   simp? [mem_def, toArr, mapIdx] at h
 --   exact Array.exists_of_mem_mapIdx h
 
 -- @[simp, grind =] theorem mem_mapIdx {b : β} {xs : NonEmptyArray α} :
 --     b ∈ mapIdx f xs ↔ ∃ (i : Nat) (h : i < xs.size), f i xs[i] = b := by
---   simp [mem_def, toArr, mapIdx, Array.mem_mapIdx]
+--   simp? [mem_def, toArr, mapIdx, Array.mem_mapIdx]
 
 -- theorem mapIdx_eq_push_iff {xs : NonEmptyArray α} {b : β} :
 --     mapIdx f xs = ys.push b ↔
 --       ∃ (a : α) (zs : NonEmptyArray α), xs = zs.push a ∧ mapIdx f zs = ys ∧ f zs.size a = b := by
---   ext <;> simp [mapIdx, toArr, Array.mapIdx_eq_push_iff]
+--   ext <;> simp? [mapIdx, toArr, Array.mapIdx_eq_push_iff]
 
 -- theorem mapIdx_eq_append_iff {xs : NonEmptyArray α} {f : Nat → α → β} {ys zs : NonEmptyArray β} :
 --     mapIdx f xs = ys ++ zs ↔
 --       ∃ (xs' : NonEmptyArray α) (zs' : NonEmptyArray α), xs = xs' ++ zs' ∧
 --         xs'.mapIdx f = ys ∧
 --         zs'.mapIdx (fun i => f (i + xs'.size)) = zs := by
---   ext <;> simp [mapIdx, toArr, Array.mapIdx_eq_append_iff]
+--   ext <;> simp? [mapIdx, toArr, Array.mapIdx_eq_append_iff]
 
 -- theorem mapIdx_eq_iff {xs : NonEmptyArray α} : mapIdx f xs = ys ↔ ∀ i : Nat, ys[i]? = xs[i]?.map (f i) := by
---   ext <;> simp [mapIdx, toArr, Array.mapIdx_eq_iff]
+--   ext <;> simp? [mapIdx, toArr, Array.mapIdx_eq_iff]
 
 -- theorem mapIdx_eq_mapIdx_iff {xs : NonEmptyArray α} :
 --     mapIdx f xs = mapIdx g xs ↔ ∀ i : Nat, (h : i < xs.size) → f i xs[i] = g i xs[i] := by
@@ -363,11 +496,11 @@ theorem mapFinIdx_singleton {a : α} {f : (i : Nat) → α → (h : i < 1) → �
 
 -- @[simp, grind =] theorem back?_mapIdx {xs : NonEmptyArray α} {f : Nat → α → β} :
 --     (mapIdx f xs).back? = (xs.back?).map (f (xs.size - 1)) := by
---   ext <;> simp [mapIdx, back?, toArr, Array.back?_mapIdx]
+--   ext <;> simp? [mapIdx, back?, toArr, Array.back?_mapIdx]
 
 -- @[simp, grind =] theorem back_mapIdx {xs : NonEmptyArray α} {f : Nat → α → β} :
 --     (xs.mapIdx f).back = f (xs.size - 1) xs.back := by
---   ext <;> simp [mapIdx, back, toArr, Array.back_mapIdx]
+--   ext <;> simp? [mapIdx, back, toArr, Array.back_mapIdx]
 
 -- @[simp, grind =] theorem mapIdx_mapIdx {xs : NonEmptyArray α} {f : Nat → α → β} {g : Nat → β → γ} :
 --     (xs.mapIdx f).mapIdx g = xs.mapIdx (fun i => g i ∘ f i) := by
@@ -376,16 +509,16 @@ theorem mapFinIdx_singleton {a : α} {f : (i : Nat) → α → (h : i < 1) → �
 
 -- theorem mapIdx_eq_replicate_iff {xs : NonEmptyArray α} {f : Nat → α → β} {b : β} :
 --     mapIdx f xs = NonEmptyArray.ofFn (fun _ => b) ↔ ∀ (i : Nat) (h : i < xs.size), f i xs[i] = b := by
---   ext <;> simp [mapIdx, toArr, Array.mapIdx_eq_replicate_iff, Array.size]
+--   ext <;> simp? [mapIdx, toArr, Array.mapIdx_eq_replicate_iff, Array.size]
 
 -- @[simp, grind =] theorem mapIdx_reverse {xs : NonEmptyArray α} {f : Nat → α → β} :
 --     xs.reverse.mapIdx f = (mapIdx (fun i => f (xs.size - 1 - i)) xs).reverse := by
---   ext <;> simp [mapIdx, reverse, toArr, Array.mapIdx_reverse, fromArray]
+--   ext <;> simp? [mapIdx, reverse, toArr, Array.mapIdx_reverse, fromArray]
 
 -- theorem toList_mapFinIdxM [Monad m] [LawfulMonad m] {xs : NonEmptyArray α}
 --     {f : (i : Nat) → α → (h : i < xs.size) → m β} :
 --     toList <$> xs.mapFinIdxM f = xs.toList.mapFinIdxM f := by
---   simp [mapFinIdxM, toList, Functor.map, pure, bind]
+--   simp? [mapFinIdxM, toList, Functor.map, pure, bind]
 --   congr
 --   funext a
 --   rw [Array.toList_mapFinIdxM]
@@ -394,6 +527,6 @@ theorem mapFinIdx_singleton {a : α} {f : (i : Nat) → α → (h : i < 1) → �
 --     {f : Nat → α → m β} :
 --     toList <$> xs.mapIdxM f = xs.toList.mapIdxM f := by
 --   rw [mapIdxM, toList_mapFinIdxM]
---   simp [List.mapIdxM]
+--   simp? [List.mapIdxM]
 
 end NonEmpty.CorrectByConstruction.Array
